src/Trace.v
@@ -1,0 +1,57 @@
+Require Import LinearScan.Lib.
+Require Import LinearScan.Context.
+Require Import LinearScan.Interval.
+Require Import LinearScan.ScanState.
+
+Set Implicit Arguments.
+Unset Strict Implicit.
+Unset Printing Implicit Defensive.
+Generalizable All Variables.
+
+Section Trace.
+
+(* These T-suffixed types and constructors are for data that is meant to be
+   exported from Coq, and so must dwell in [Set]. *)
+
+Definition IntervalIdT : Set := nat.
+Definition PhysRegT : Set := nat.
+
+Inductive SpillConditionT : Set :=
+  | NewToHandledT       of IntervalIdT
+  | UnhandledToHandledT of IntervalIdT
+  | ActiveToHandledT    of IntervalIdT & PhysRegT
+  | InactiveToHandledT  of IntervalIdT & PhysRegT.
+
+Inductive SplitPositionT : Set :=
+  | BeforePosT of nat
+  | EndOfLifetimeHoleT of nat.
+
+Definition TrueIfActiveT : Set := bool.
+
+Inductive SSTrace : Set :=
+  | ESplitAssignedIntervalForReg of PhysRegT
+  | ESplitActiveOrInactiveInterval of TrueIfActiveT
+  | EIntervalHasUsePosReqReg of IntervalIdT
+  | EIntervalBeginsAtSplitPosition
+  | EMoveUnhandledToActive of PhysRegT
+  | ESplitActiveIntervalForReg of PhysRegT
+  | ESplitAnyInactiveIntervalForReg of PhysRegT
+  | ESpillInterval of SpillConditionT
+  | ESpillCurrentInterval
+  | ESplitUnhandledInterval
+  | ESplitCurrentInterval of SplitPositionT
+  | ETryAllocateFreeReg of IntervalIdT
+  | EAllocateBlockedReg of IntervalIdT
+  | ERemoveUnhandledInterval of IntervalIdT
+  | ECannotInsertUnhandled
+  | EIntervalBeginsBeforeUnhandled of IntervalIdT
+  | ENoValidSplitPosition of IntervalIdT
+  | ECannotSplitSingleton of IntervalIdT
+  | ERegisterAlreadyAssigned of PhysRegT
+  | ERegisterAssignmentsOverlap of PhysRegT
+  | EUnexpectedNoMoreUnhandled
+  | ECannotSpillIfRegisterRequired of PhysRegT
+  | EFuelExhausted
+  | ENotYetImplemented of nat.
+
+End Trace.
